add formatting, service invariants, and some progress on lemma_BCE_Validity_Correct_Nodes_Decide_Codeword

bce/bce_proof.dfy
@@ -6,6 +6,9 @@ import opened BCE_Protocol_Service
 import opened BCE_Protocol_Node
 
 
+/****************************************************************************************/
+/*                                   Equivalence                                        */
+/****************************************************************************************/ 
 lemma lemma_BCE_Equivalence(s:Service, s':Service, s'':Service) 
     requires BCE(s, s', s'');
     ensures forall node :: 
@@ -14,6 +17,11 @@ lemma lemma_BCE_Equivalence(s:Service, s':Service, s'':Service)
         node.decision == Codeword;
 {}
 
+
+/****************************************************************************************/
+/*                                  Termination                                         */
+/****************************************************************************************/ 
+
 lemma lemma_BCE_Termination(s:Service, s':Service, s'':Service) 
     requires BCE(s, s', s'');
     ensures forall node :: 
@@ -21,6 +29,11 @@ lemma lemma_BCE_Termination(s:Service, s':Service, s'':Service)
         ==> 
         (node.decision == Codeword || node.decision == Bottom);
 {}
+
+
+/****************************************************************************************/
+/*                                     Validity                                         */
+/****************************************************************************************/ 
 
 /*
 - At the end of round 1: >= n-f symbols in Symbols are common, v;
@@ -41,6 +54,7 @@ lemma lemma_BCE_Validity(s:Service, s':Service, s'':Service)
             ==> 
             node.decision == Codeword);
 {
+    lemma_Service_Maintains_Invariants(s, s', s'');
     lemma_BCE_Validity_Receive_n_f_Common_Symbols(s, s');
     assert forall node :: node in s'.nodes && !node.faulty ==> node.state == Phase2;
     var syndromes := syndromesToExchange(s'.nodes);
@@ -58,11 +72,82 @@ lemma lemma_BCE_Validity_Receive_n_f_Common_Symbols(s:Service, s':Service)
         node.symbols == node.codeword;
 {}
 
+
+// TONY
 lemma lemma_BCE_Validity_Correct_Nodes_Decide_Codeword(s':Service, syndromes: seq<seq<syndrome>>) 
+    requires node_invariants(s');
+    requires forall node :: node in s'.nodes ==> node.n == |node.symbols| == |node.codeword|;
+    requires syndromes == syndromesToExchange(s'.nodes);
+    requires |syndromes| == s'.n;
     requires forall node :: 
-        && node in s'.nodes && !node.faulty
+        node in s'.nodes && !node.faulty
         ==>
-        node.symbols == node.codeword;
-    ensures forall node :: node in s'.nodes && !node.faulty ==> decideOnCodeWord(node, syndromes[node.id]);
+        && node.symbols == node.codeword
+        && node.state == Phase2
+        && 0 <= node.id < s'.n
+        && 0 <= node.id < |syndromes[node.id]|;
+    ensures forall node :: 
+        node in s'.nodes && !node.faulty ==> decideOnCodeWord(node, syndromes[node.id]);
+{
+    lemma_Exchanged_Syndromes_Are_Extracted(s'.nodes);
+    forall node | node in s'.nodes && !node.faulty
+    ensures decideOnCodeWord(node, syndromes[node.id])
+    {
+        var syndromes_received := syndromes[node.id];
+        var my_syndrome := syndromes_received[node.id];
+        assert my_syndrome == computeSyndrome(node);
+        lemma_Computed_Syndromes_Have_Length_n(node, my_syndrome);
+        lemma_BCE_Validity_Correct_Nodes_Own_Syndrome_Is_Good(node, my_syndrome);
+        assert countTrue(syndromes_received[node.id]) >= node.n - node.f;
+        assert countGoodSyndromes(syndromes_received, node.n-node.f) >= node.n - node.f;
+    }
+}
+
+
+lemma {:induction my_syndrome} lemma_BCE_Validity_Correct_Nodes_Own_Syndrome_Is_Good(node: Node, my_syndrome: syndrome) 
+    requires !node.faulty;
+    requires node.state == Phase2;
+    requires |my_syndrome| == node.n;
+    requires node.n == 3 * node.f + 1
+    ensures countTrue(my_syndrome) >= node.n - node.f;
+{
+
+}
+
+
+/****************************************************************************************/
+/*                                Service Invariants                                    */
+/****************************************************************************************/ 
+
+predicate node_invariants(s: Service)
+{
+    forall node :: node in s.nodes && !node.faulty ==>
+    && node.n == node.f * 3 + 1
+    && 0 <= node.id < node.n
+    && 0 <= node.id < node.n
+    && |node.codeword| == node.n
+    && node.n == s.n
+    && node.f == s.f
+}
+
+predicate service_invariants(s:Service, s':Service, s'':Service)
+{
+    BCE(s, s', s'')
+    ==>
+    && serviceInit(s)
+    && node_invariants(s) && node_invariants(s') && node_invariants(s'')
+    && s.f == s'.f == s''.f
+    && s.n == s'.n == s''.n
+    // num of nodes is constant
+    && |s.nodes| == |s'.nodes| == |s''.nodes| == s.n
+    // correctness of each node is constant
+    && (forall  id :: 0 <= id < s.n ==> s.nodes[id].faulty == s'.nodes[id].faulty == s''.nodes[id].faulty)
+    // id of each correct node is constant
+    && (forall  i :: 0 <= i < s.n && !s.nodes[i].faulty ==> s.nodes[i].id == i)
+}
+
+lemma lemma_Service_Maintains_Invariants(s:Service, s':Service, s'':Service) 
+    requires BCE(s, s', s'');
+    ensures service_invariants(s, s', s'');
 {}
 }
